Liveness.i.dfy
@@ -1,0 +1,27 @@
+include "Temporal.s.dfy"
+include "Lift.i.dfy"
+
+module Temporal__Liveness_i {
+    import opened Temporal__Temporal_s
+    import opened Temporal__Lift_i
+
+    // f happens infinitely often.
+    // once g happens, it is stable until h
+    // f && g ==> h
+    // thus g leadsto h
+    //  (because g stays true until f happens, at which point f&&g==>h.)
+    lemma InferFromUntil(f:temporal, g:temporal, h:temporal)
+        requires sat(always(eventually(f)))
+        requires sat(always(until(g, h)))
+        requires sat(always(implies(and(f, g), h)))
+        ensures sat(leadsto(g, h))
+    {
+    }
+
+    lemma InferInfinitelyOften(f:temporal, g:temporal)
+        requires sat(always(eventually(f)))
+        requires sat(leadsto(f, g))
+        ensures sat(always(eventually(g)))
+    {
+    }
+}
